Types.v
@@ -2,10 +2,11 @@ Add LoadPath "vst".
 
 Require Import Coq.Unicode.Utf8.
 Require Import msl.eq_dec.
-Require Import Language.
-Require Import List.
-Import ListNotations.
 Require Import Subst.
+Require Export Language.
+Require Import List.
+Require Import ListSet.
+Import ListNotations.
 
 Definition vv : var := V 0.
 
@@ -27,7 +28,7 @@ Definition base_of_type b :=
 Definition base_of_val (v: value) :=
   match v with
     | int_v  _ => int_t
-    | loc_v  l => ref_t l
+    | loc_v l => ref_t l
     | null     => null_t
   end.
 
@@ -104,6 +105,7 @@ Definition subst_r s reft :=
 
 Instance Subst_reft_var : Subst reft_type var var := subst_r_var.
 Instance Subst_reft : Subst reft_type var expr := subst_r.
+Instance subst_reft_loc : Subst reft_type loc loc := subst_r_loc.
 
 Definition type_binding : Set := (var * reft_type)%type.
 
@@ -117,7 +119,21 @@ Notation "{ vv : t | P }" := (dummyt vv t P%reft) (at level 0, vv at level 99, n
 (** Environments **)
 Definition bind_env (B T : Set) : Set := list (B * T)%type.
 Definition type_env : Set := bind_env var reft_type.
-Definition heap_env : Set := bind_env loc (var * reft_type)%type.
+Definition heap_env : Set := list (loc * type_binding)%type.
+
+Fixpoint subst_heap_var s (h : heap_env) : heap_env :=
+  match h with
+    | nil => nil
+    | (l, xt) :: h' => (l, subst s xt) :: subst_heap_var s h'
+  end.
+
+Instance Subst_heap_var : Subst heap_env var var := subst_heap_var.
+
+Fixpoint subst_heap_loc s (h : heap_env) : heap_env :=
+  match h with
+    | nil => nil
+    | (l, (x, t)) :: h' => (subst s l, (x, subst s t)) :: subst_heap_loc s h'
+  end.
 
 (** Procedures **)
 Record proc_schema : Set :=
@@ -127,16 +143,26 @@ Record proc_schema : Set :=
              s_heap_out: heap_env;
              s_ret: type_binding }.
 
-Definition subst_schema (s S :=
-  let subst_both s xt := (subst s (fst xt), subst s (snd xt)) in
+Definition subst_schema (s : var -> var) S :=
+  let subst_both s xt := (@subst _ _ _ Subst_var_var s (fst xt),
+                          @subst _ _ _ Subst_reft_var s (snd xt)) in
   match S with
     | mkSchema xs ts hi ho xt =>
-      mkSchema (subst s xs) (subst s ts) (subst s hi) (subst s ho) (subst_both s xt)
+      mkSchema (subst s xs) (subst s ts) (subst_heap_var s hi) (subst_heap_var s ho) (subst_both s xt)
   end.
 
-Definition 
+Definition subst_schema_loc (s : loc -> loc) S :=
+  match S with
+    | mkSchema xs ts hi ho (x, t) =>
+      mkSchema xs (subst s ts) (subst_heap_loc s hi) 
+               (subst_heap_loc s ho) (x, subst s t)
+  end.
 
 Instance Subst_proc_schema : Subst proc_schema var var := subst_schema.
+Instance Subst_proc_schema_loc : Subst proc_schema loc loc := subst_schema_loc.
+
+Instance Subst_binding_loc : Subst type_binding loc loc := 
+  fun s xt => (fst xt, subst s (snd xt)).
 
 Definition proc_env : Type := bind_env pname (stmt * proc_schema)%type.
 
@@ -163,6 +189,12 @@ Definition fun_in : (pname * (stmt * proc_schema)) -> proc_env -> Prop :=
 
 Definition fun_not_in : pname  -> proc_env -> Prop :=
   fun f Φ => Forall (fun ft => fst ft <> f) Φ.
+
+Definition heap_split Σ1 Σ2 Σ :=
+  forall l, 
+    (loc_in l Σ /\ 
+     ((loc_in l Σ1 /\ loc_not_in l Σ2) \/ (loc_in l Σ2 /\ loc_not_in l Σ1))
+     \/ (loc_not_in l Σ /\ loc_not_in l Σ1 /\ loc_not_in l Σ2)).
 
 Notation "X ∈ Y" := (In X Y) (at level 40).
 
@@ -201,3 +233,115 @@ Proof.
 Qed.
 
 Definition ν := vv.
+
+Hint Rewrite Forall_forall.
+Hint Unfold heap_split loc_not_in loc_in : heap.
+
+Theorem loc_in_dec :
+  forall l Σ, {loc_in l Σ} + {~ loc_in l Σ}.
+Proof.
+  intros.
+  unfold loc_in.
+  induction Σ.
+  right. intuition. destruct H. inversion H.
+  destruct IHΣ.
+  left. destruct e. exists x. right. assumption.
+  intuition.
+  cut ({l = a0} + {l <> a0}). intro.
+  destruct H. 
+    rewrite <- e in *.
+    left. exists b. left. reflexivity.
+    right. intro. apply n.
+    destruct H.
+    destruct H. inversion H. subst.
+    congruence.
+    exists x. assumption.
+  apply eq_dec.
+Qed.
+
+Lemma loc_in_not_in :
+  forall Σ l,
+    ~loc_in l Σ <-> loc_not_in l Σ.
+Proof.
+  intro Σ.
+  unfold loc_not_in.
+  unfold loc_in.
+  induction Σ.
+  intros.
+  rewrite Forall_forall.
+  constructor.
+  intros.
+  inversion H0.
+  intros.
+  intro. 
+  destruct H0.
+  inversion H0.
+  constructor.
+  intros.
+  destruct (IHΣ l).
+  rewrite Forall_forall in *.
+  intros.
+  destruct H2. subst.
+  intuition.
+  destruct x. subst. 
+  apply H.
+  exists t. left. reflexivity.
+  apply H0.
+  intro.
+  apply H.
+  destruct H3.
+  exists x0. apply in_cons. assumption. assumption.
+  intros.
+  intro.
+  destruct (IHΣ l).
+  rewrite Forall_forall in *.
+  destruct H0.
+  destruct H0.
+  destruct a. inversion H0. subst.
+  specialize (H (l,x)). apply H. left. reflexivity. reflexivity.
+  apply H2. intros.
+  apply H. apply in_cons. assumption. exists x. assumption.
+Qed. (** OOF **)
+
+Lemma heap_split_comm :
+  forall Σ1 Σ2 Σ,
+    heap_split Σ1 Σ2 Σ ->
+    heap_split Σ2 Σ1 Σ.
+Proof.
+  intros.
+  unfold heap_split in *.
+  intros. 
+  destruct (H l); firstorder.
+Qed.
+
+Lemma heap_split_emp :
+  forall l Σ1 Σ2 Σ,
+    heap_split Σ1 Σ2 Σ ->
+    loc_not_in l Σ ->
+    loc_not_in l Σ1.
+Proof.
+  intros.
+  unfold heap_split in H.
+  specialize (H l).
+  rewrite <- loc_in_not_in in *.
+  destruct H.
+  destruct H.
+  congruence.
+  destruct H. destruct H1.
+  rewrite <- loc_in_not_in in *.
+  assumption.
+Qed.
+
+Lemma heap_split_emp' :
+  forall l Σ1 Σ2 Σ,
+    heap_split Σ1 Σ2 Σ ->
+    loc_not_in l Σ ->
+    loc_not_in l Σ2.
+Proof.
+  intros.
+  apply heap_split_comm in H.
+  eapply heap_split_emp;
+  eauto.
+Qed.
+
+Hint Resolve heap_split_emp heap_split_emp' loc_in_not_in : heaps.
